Switch traces to be inductive; start of principled refinement automation via normalization

Refinement.v
@@ -1,4 +1,4 @@
-Require Import Process Eqdep_dec.
+Require Import List Process Eqdep_dec.
 
 
 Ltac inv H := inversion H; clear H; subst;
@@ -10,254 +10,225 @@ Ltac inv H := inversion H; clear H; subst;
 Section Refinement.
   Variable chs : channels.
 
-  Theorem refines_refl : forall k,
-    refines (chs := chs) k k.
+  (** A normal form for processes *)
+
+  CoInductive proc0 :=
+  | NSend (ch : channel) (v : chs ch) (k : proc0)
+  | NRecv (ch : channel) (k : chs ch -> proc0)
+  | NDone.
+
+  Record proc := {
+    Chans : direction * channel -> Prop;
+    Code : proc0
+  }.
+
+  Definition procs := list proc.
+
+  CoFixpoint proc0D (p : proc0) : process chs :=
+    match p with
+    | NSend ch v k => DoSend ch v (proc0D k)
+    | NRecv ch k => DoRecv ch (fun v => proc0D (k v))
+    | NDone => Done
+    end.
+
+  Definition procD (p : proc) : process chs :=
+    Restrict (Chans p) (proc0D (Code p)).
+
+  Fixpoint procsD (ps : procs) : process chs :=
+    match ps with
+    | nil => Done
+    | p :: ps' => Parallel (procD p) (procsD ps')
+    end.
+
+  Definition norm (p : process chs) (ps : procs) : Prop :=
+    refines p (procsD ps)
+    /\ refines (procsD ps) p.
+
+  Theorem normDone : norm Done ({| Chans := fun _ => True; Code := NDone |} :: nil).
   Proof.
-    intros; hnf; eauto.
+    split; simpl; do 2 intro.
+    eauto.
+    inv H; eauto.
+    inv H3; eauto.
+    rewrite (expand_ok (procD
+            {| Chans := fun _ : direction * channel => True; Code := NDone |})) in H2; simpl in H2.
+    inv H2; eauto.
+    rewrite (expand_ok (proc0D NDone)) in H1; simpl in H1.
+    inv H1; eauto.
+    inv H5; eauto.
+    inv H5; eauto.
   Qed.
 
-  Theorem done_left : forall k,
-    refines (chs := chs) Done k.
+  Lemma interleave_sym : forall tr1 tr2 tr3,
+    interleave (chs := chs) tr1 tr2 tr3
+    -> interleave tr2 tr1 tr3.
   Proof.
-    intros; hnf; intros.
+    induction 1; eauto.
+  Qed.
+
+  Theorem Parallel_comm : forall p1 p2,
+    refines (chs := chs) (p1 || p2) (p2 || p1).
+  Proof.
+    do 4 intro.
+    inv H; eauto using interleave_sym.
+  Qed.
+
+  Ltac reassoc1 :=
+    try match goal with
+        | [ H : _ :: _ = _ :: _ |- _ ] => injection H; clear H; intros; subst
+        end;
+    try match goal with
+        | [ IHinterleave : forall tr3 tr3 : trace chs, _, H : interleave _ _ _ |- _ ] =>
+          apply IHinterleave in H; clear IHinterleave; firstorder
+        end;
+    try match goal with
+        | [ H : _ = _ -> ex _ |- _ ] => destruct H; intuition; []
+        end;
+    try solve [ do 2 esplit; [ solve [ econstructor; eauto | apply IntCons2; eauto ] | eauto ] ].
+
+  Ltac induct :=
+    match goal with
+    | [ H : interleave _ _ ?ls |- _ ] =>
+      remember ls; induction H; subst; eauto; try congruence
+    end.
+
+  Ltac reassoc := solve [ reassoc1 ] || (induct; reassoc1).
+
+  Lemma interleave_reassoc1 : forall tr3 tr tr',
+    interleave (chs := chs) tr3 tr tr'
+    -> forall tr1 tr2, interleave (chs := chs) tr1 tr2 tr
+    -> exists tr'', interleave tr3 tr1 tr'' /\ interleave tr'' tr2 tr'.
+  Proof.
+    induction 1; eauto; intros; reassoc.
+  Qed.
+
+  Theorem Parallel_assoc1 : forall p1 p2 p3,
+    refines (chs := chs) (p1 || (p2 || p3)) ((p1 || p2) || p3).
+  Proof.
+    do 5 intro.
+    inv H; eauto.
+    inv H3; eauto.
+    eapply interleave_reassoc1 in H7; try apply H5; firstorder.
+    eauto.
+  Qed.
+
+  Lemma interleave_reassoc2 : forall tr3 tr tr',
+    interleave (chs := chs) tr tr3 tr'
+    -> forall tr1 tr2, interleave (chs := chs) tr1 tr2 tr
+    -> exists tr'', interleave tr2 tr3 tr'' /\ interleave tr1 tr'' tr'.
+  Proof.
+    induction 1; eauto; intros; reassoc.
+  Qed.
+
+  Theorem Parallel_assoc2 : forall p1 p2 p3,
+    refines (chs := chs) ((p1 || p2) || p3) (p1 || (p2 || p3)).
+  Proof.
+    do 5 intro.
+    inv H; eauto.
+    inv H2; eauto.
+    eapply interleave_reassoc2 in H7; try apply H5; firstorder eauto.
+  Qed.
+
+  Lemma procsD_app1 : forall ps2 ps1,
+    refines (procsD (ps1 ++ ps2)%list) (Parallel (procsD ps1) (procsD ps2)).
+  Proof.
+    induction ps1; simpl; hnf; intros; eauto.
+    apply Parallel_assoc1.
     inv H; eauto.
   Qed.
 
-  Theorem done_right : forall k k',
-    refines k k'
-    -> refines (chs := chs) k (Done || k').
+  Lemma interleave_nil1' : forall nl tr1 tr2,
+    interleave (chs := chs) nl tr1 tr2
+    -> nl = nil
+    -> tr1 = tr2.
   Proof.
-    intros; hnf; intros.
-    apply H in H0; firstorder.
-    eexists; split.
-    econstructor.
-    eauto.
-    eauto.
-    eauto.
-    auto.
-  Qed.
-
-  Theorem recv_recv : forall ch k k' k'',
-    (forall v, refines (k v) (k' v || k''))
-    -> refines (DoRecv (chs := chs) ch k) (DoRecv ch k' || k'').
-  Proof.
-    intros; hnf; intros.
-    inv H0; eauto.
-
-    apply H in H4; firstorder.
-    eexists; split.
-    inv H0.
-    econstructor.
-    econstructor.
-    eauto.
-    eauto.
-    econstructor; eauto.
-    econstructor.
-    econstructor.
-    econstructor.
-    econstructor.
-    eauto.
-    eauto.
-  Qed.
-
-  Lemma traceEqual_interleave : forall tr tr',
-    traceEqual (chs := chs) tr' tr
-    -> forall tr1 tr2, interleave tr1 tr2 tr
-    -> interleave tr1 tr2 tr'.
-  Proof.
-    cofix; destruct 2.
-
-    destruct H.
-    constructor.
-    econstructor; eauto.
-
-    destruct H.
-    constructor.
-    econstructor; eauto.
-
-    inv H.
-    eauto.
-
-    inv H.
-    eauto.
-
-    eauto.
-    eauto.
-  Qed.
-
-  Hint Immediate traceEqual_interleave.
-
-  Theorem recv_recv_restricted : forall (which : direction * channel -> Prop) ch k k' k'',
-    which (Recv, ch)
-    -> (forall v, refines (k v) (Restrict which (k' v) || k''))
-    -> refines (DoRecv (chs := chs) ch k) (Restrict which (DoRecv ch k') || k'').
-  Proof.
-    intros; hnf; intros.
-    inv H1; eauto.
-
-    apply H0 in H5; clear H0; firstorder.
-    inv H0.
-    Focus 2.
-
-    inv H1.
-    eexists; split.
-    econstructor.
-    econstructor.
-    econstructor.
-    econstructor.
-    eauto.
-    eauto.
-    eauto.
-    eauto.
-
-    inv H4.
-    Focus 2.
-    eexists; split.
-    econstructor.
-    econstructor.
-    econstructor.
-    econstructor.
-    eauto.
-    eauto.
-    2: eauto.
-    eauto.
-
-    eexists; split.
-    econstructor.
-    econstructor.
-    econstructor.
-    eauto.
-    eauto.
-    eauto.
-    econstructor; eauto.
-    eauto.
-  Qed.
-
-  Theorem match_right : forall ch k k' k'' v,
-    refines k (k' || k'' v)
-    -> refines (chs := chs) k (DoSend ch v k' || DoRecv ch k'').
-  Proof.
-    intros; hnf; intros.
-    apply H in H0; firstorder.
-    inv H0; subst.
-    Focus 2.
-    inv H1; eauto.
-
-    eexists; split.
-    econstructor.
-    econstructor.
-    eauto.
-    econstructor.
-    eauto.
-    eauto.
-    auto.
+    induction 1; simpl; intros; intuition; try congruence.
   Qed.
 
   Lemma interleave_nil1 : forall tr1 tr2,
-    interleave (chs := chs) SNil tr1 tr2
-    -> traceEqual tr1 tr2.
+    interleave (chs := chs) nil tr1 tr2
+    -> tr1 = tr2.
   Proof.
-    cofix; inversion 1; subst; intros.
-    eauto.
-    eauto.
-    constructor; eauto.
+    eauto using interleave_nil1'.
   Qed.
 
-  Lemma traceEqual_sym : forall tr1 tr2,
-    traceEqual (chs := chs) tr1 tr2
-    -> traceEqual tr2 tr1.
+  Lemma procsD_app2 : forall ps2 ps1,
+    refines (Parallel (procsD ps1) (procsD ps2)) (procsD (ps1 ++ ps2)%list).
   Proof.
-    cofix; destruct 1; econstructor; eauto.
+    induction ps1; simpl; hnf; intros; eauto.
+
+    inv H; eauto.
+    inv H2; eauto.
+    apply interleave_nil1 in H5; congruence.
+
+    apply Parallel_assoc2 in H.
+    inv H; eauto.
   Qed.
 
-  Lemma traceEqual_trans : forall tr1 tr2 tr3,
-    traceEqual (chs := chs) tr1 tr2
-    -> traceEqual tr2 tr3
-    -> traceEqual tr1 tr3.
+  Theorem normParallel : forall p1 ps1 p2 ps2, norm p1 ps1
+    -> norm p2 ps2
+    -> norm (Parallel p1 p2) (ps1 ++ ps2)%list.
   Proof.
-    cofix; destruct 1; inversion 1; econstructor; eauto.
-  Qed.
+    split; simpl; do 2 intro.
 
-  Theorem match_right_restricted : forall (which : _ -> Prop) ch k k' k'' v,
-    which (Send, ch)
-    -> refines k (Restrict which k' || k'' v)
-    -> refines (chs := chs) k (Restrict which (DoSend ch v k') || DoRecv ch k'').
-  Proof.
-    intros; hnf; intros.
-    apply H0 in H1; clear H0; firstorder.
-    inv H0; subst.
-    Focus 2.
+    apply procsD_app2.
+    unfold norm, refines in *.
+    intuition.
     inv H1; eauto.
 
+    apply procsD_app1 in H1.
+    unfold norm, refines in *.
+    intuition.
+    inv H1; eauto.
+  Qed.
+
+  Theorem normSend : forall ch v k p,
+    norm k (p :: nil)
+    -> Chans p (Send, ch)
+    -> norm (DoSend ch v k) ({| Chans := Chans p; Code := NSend ch v (Code p) |} :: nil).
+  Proof.
+    unfold norm, refines; simpl; intuition.
+
+    inv H; eauto.
+    apply H1 in H7; clear H1.
+    inv H7; eauto.
     inv H4.
-    Focus 2.
-    apply interleave_nil1 in H7.
-    eexists; split.
+    apply interleave_sym in H6; apply interleave_nil1 in H6; subst.
+    unfold procD in *; simpl in *.
+    inv H3; eauto.
     econstructor.
+    2: eauto.
+    2: eauto.
     econstructor.
-    econstructor.
+    rewrite (expand_ok (proc0D (NSend ch v (Code p)))); simpl.
     eauto.
     eauto.
     econstructor.
+    2: eauto.
+    2: eauto.
+    econstructor.
+    rewrite (expand_ok (proc0D (NSend ch v (Code p)))); simpl.
     eauto.
     eauto.
-    eauto using traceEqual_trans, traceEqual_sym.
+    econstructor.
+    2: eauto.
+    2: eauto.
+    econstructor.
+    simpl.
+    rewrite (expand_ok (proc0D (NSend ch v (Code p)))); simpl.
+    eauto.
+    eauto.
 
-    eexists; split.
-    econstructor.
-    econstructor.
-    econstructor.
-    eauto.
-    eauto.
+    unfold procD in *; simpl in *.
+    inv H; eauto.
+    inv H6.
+    apply interleave_sym in H8; apply interleave_nil1 in H8; subst.
+    inv H5; eauto.
+    rewrite (expand_ok (proc0D (NSend ch v (Code p)))) in *.
+    simpl in *.
+    inv H4; eauto.
     econstructor; eauto.
-    eauto.
-    auto.
-  Qed.
-
-  Theorem send_send : forall ch k k' k'' v,
-    refines k (k' || k'')
-    -> refines (DoSend (chs := chs) ch v k) (k' || DoSend ch v k'').
-  Proof.
-    intros; hnf; intros.
-    inv H0; eauto.
-    apply H in H5; clear H; firstorder.
-    inv H.
-    Focus 2.
-
-    inv H0.
-    eexists; split.
-    econstructor.
-    eauto.
-    econstructor.
-    eauto.
-    eauto.
-    eauto.
-
-    eexists; split.
-    econstructor.
-    eauto.
-    econstructor.
-    eauto.
-    econstructor; eauto.
-    eauto.
-  Qed.
-
-  Theorem done_right_restricted : forall which k k',
-    refines k k'
-    -> refines (chs := chs) k (Restrict which Done || k').
-  Proof.
-    intros; hnf; intros.
-    apply H in H0; firstorder.
-    eexists; split.
-    econstructor.
-    econstructor.
-    eauto.
-    eauto.
-    eauto.
-    eauto.
-    auto.
+    apply H2.
+    inv H7; eauto.
   Qed.
 End Refinement.
-
-Ltac refines := repeat (apply refines_refl || apply done_left || apply done_right
-                              || apply recv_recv || apply match_right; intros).
